raft/simulator/lib/Simulator.ml
@@ -1,0 +1,100 @@
+open Colors
+open Prelude
+open RsaKeyFun
+open Core
+
+(* the generic type *)
+type ('a, 'b) idrep = { id : 'a ; replica : 'b }
+
+(* create a list of replicas *)
+class ['a, 'b] replicas = object(self)
+  val mutable r : ('a, 'b) idrep list ref = ref []
+
+  (* assign replicas *)
+  method set_replicas (l : ('a, 'b) idrep list) =
+    r := l
+
+  method get_replicas : ('a, 'b) idrep list =
+    !r
+
+  method find_replica id : ('a, 'b) idrep option =
+    List.find ~f:(fun x -> id = x.id) !r
+
+  method replace_replica id rep : unit =
+    r := List.map ~f:(fun x -> if id = x.id then { id = id; replica = rep } else x) !r
+end
+
+(* print error messages *)
+let print_err msg =
+  print_endline (kBRED ^ "Error:\t[" ^ msg ^ "]" ^ kNRM)
+
+(* print info messages with c - color; t - message type; msg - message *)
+let print_info c t msg =
+  print_endline (c ^ "Info:\t{" ^ t ^ ": " ^ msg ^ "}" ^ kNRM)
+
+(* print results t - timestamp; d - elapsed time; avg - average *)
+let print_res t d avg  =
+  print_endline (kMAG ^ "Result:\t[Timestamp: " ^ string_of_int t
+                 ^ "; elapsed time: " ^ (Batteries.String.of_list (Prelude.Time.time2string d))
+                 ^ "; average: " ^ Batteries.String.of_list (Prelude.Time.time2string avg)
+                 ^ "]" ^ kNRM)
+
+
+type ('a) run_conf = {
+  version : string;
+  protocol : string;
+  client_id : int;
+  private_key : Nocrypto.Rsa.priv;
+  primary : 'a;
+}
+
+class virtual ['a, 'b] runner c = object(self)
+  val mutable conf : ('a) run_conf = c
+
+  (** create all the replicas **)
+  method virtual create_replicas : unit
+
+  (** specify how some client request is made **)
+  method virtual mk_request : int -> int -> 'b
+
+  (** specify the client **)
+  method virtual run_client : int -> int -> Prelude.Time.t -> int -> unit
+
+  (* maybe this could be more generalized *)
+  (** An implementation should catch the spec args <max> <printing_period> initialize the crypto;
+      set the replicas and at last call run_client **)
+  method callback : int -> int -> unit -> unit =
+    (fun max printing_period () ->
+       print_info (kBLU) "Main" "Initialize random generator";
+       let () = Nocrypto_entropy_unix.initialize () in
+
+       print_info (kBLU) "Main" "Start replicas";
+       self#create_replicas;
+
+       print_info (kBLU) "Main" "Fire up client";
+       let initial_timestamp = 1 in
+       let initial_avg       = Prelude.Time.mk_time 0. in
+       self#run_client initial_timestamp max initial_avg printing_period)
+
+
+  (** the default cli specification **)
+  method spec : Command.t =
+    let () = Nocrypto_entropy_unix.initialize () in
+    Command.basic_spec
+      ~summary:"Start a client"
+      Command.Spec.(
+        empty
+        +> flag "-max" (optional_with_default 10 int)
+          ~doc:" Number of messages to send (default 10)"
+
+        +> flag "-printing-period" (optional_with_default 10 int)
+          ~doc:" Number of messages till a summary is printed (default 10)"
+      )
+      self#callback
+
+  (** run a simulator with some specified configuration **)
+  method run =
+    print_info (kWHT) "Main" ("Running simulator for " ^ conf.protocol
+                              ^ " Version: " ^ conf.version);
+    Command.run ~version:conf.version ~build_info:conf.protocol self#spec
+end
