raft/simulator/pb/PbSimul.ml
@@ -1,0 +1,140 @@
+open Colors
+open Prelude
+open PbReplicaEx
+open RsaKeyFun
+open Core
+open Simulator
+
+(* turn this to false if you don't want to sign messages *)
+let signing : bool ref = ref true
+
+(* convert the node name to string *)
+let node2string n =
+  match (Obj.magic n) with
+  | PBprimary -> "Primary "
+  | PBbackup -> "Backup "
+  | _ -> "Other "
+
+(* create a new replica *)
+let to_replica n =
+  print_info (kBLU) "Main" ("Starting " ^ (String.of_char_list (name2string n)));
+  { id = Obj.magic n; replica = local_replica (Obj.magic n) }
+
+(* init the replicas object *)
+let r = new replicas
+
+let sign_request breq priv =
+  let o  = Obj.magic (PBinput breq) in
+  sign_one o priv
+
+(* build the request destination *)
+(* let destination2string (n : name) : string =
+ *   match Obj.magic n with
+ *   | PBprimary -> "P(" ^ string_of_int (Obj.magic 0) ^ ")"
+ *   | PBbackup -> "B(" ^ string_of_int (Obj.magic 0) ^ ")"
+ *   | PBc -> "C(" ^ string_of_int (Obj.magic 0) ^ ")" ;; *)
+
+let print_msgs msgs =
+  List.fold_right ~f:(fun acc x -> acc ^ ";" ^ x) (List.map ~f:(fun x -> (String.of_char_list (directedMsg2string x))) msgs)
+
+(* run the replicas on some input *)
+let rec run_replicas_on_inputs (inflight : directedMsgs) : directedMsgs =
+  print_info (kMAG) "Queue" ((print_msgs inflight) "");
+  (* check if there is some message in queue *)
+  match inflight with
+  | [] ->
+    print_info (kBLU) "Main" "All messages processed stopping";
+    []
+  | dm :: dms ->
+    (* we have some message and now we iterate through all its destinations *)
+    match dm.dmDst with
+    (* restart loop if there a no destinations *)
+    | [] -> run_replicas_on_inputs dms
+    | id :: ids ->
+      print_info (kCYN) "Procesing" ((String.of_char_list (directedMsg2string dm)));
+      (* create a new message without the taken id *)
+      let dm' = { dmMsg = dm.dmMsg; dmDst = ids; dmDelay = dm.dmDelay } in
+      (* find the replica mathing the id *)
+      match r#find_replica id with
+      | None ->
+        print_err ("Couldn't find id " ^ node2string id);
+        let failed_to_deliver = { dmMsg = dm.dmMsg; dmDst = [id]; dmDelay = dm.dmDelay } in
+        (* requeue message which failed to deliver ? *)
+        failed_to_deliver :: run_replicas_on_inputs (dm' :: dms)
+      | Some rep ->
+        (* we have found the replica *)
+        print_info (kGRN) ((node2string rep.id) ^ "got") (String.of_char_list (msg2string (Obj.magic dm.dmMsg)));
+        (* run the state machine on the message input *)
+        let (rep',dmsgs) = lrun_sm rep.replica (Obj.magic dm.dmMsg) in
+        print_info (kCYN) (node2string id ^ "State transistion completed") ("Return " ^ (String.of_char_list (directedMsgs2string dmsgs)));
+        (* replace the state machine of the replica *)
+        print_info (kCYN) (node2string id) (Obj.magic rep.replica);
+        r#replace_replica id rep';
+        (* (message without current replica) :: (next messages) @ (newly created messages) *)
+        run_replicas_on_inputs (dm' :: dms @ dmsgs)
+
+(* implement the virtual simulator *)
+class ['a, 'b] pb c = object(self)
+  inherit ['a, 'b] runner c
+
+  (* create the replication system with one primary and three backups *)
+  method create_replicas =
+    r#set_replicas [to_replica PBprimary; to_replica PBbackup]
+
+  (* create a client request *)
+  method mk_request (timestamp : int) (request : int) =
+    PBinput request
+    (* let opr       = Obj.magic (Opr_add request) in
+     * let breq      = Bare_req (opr,timestamp,(Obj.magic c.client_id)) in
+     * let tokens    = [ (if !signing then Obj.magic (sign_request breq c.private_key) else Obj.magic()) ] in
+     * PBFTrequest (Req(breq,tokens)) *)
+
+
+  (* run the client recursively
+   * timestamp - is the current term and gets inc every round
+   * max - the maximum rounds to go
+   * avg - an ongoing calculated average
+   * printing_period - the number of timestamps before printing some results *)
+  method run_client timestamp max avg printing_period =
+    (* generate request number *)
+    let rand = Random.int 20 in
+    (* create a simple PNinput request *)
+    let req = self#mk_request (Obj.magic timestamp) rand in
+    (* create a message list with the primary as destination *)
+    let inflight = [{ dmMsg = Obj.magic req; dmDst = [c.primary]; dmDelay = 0 }] in
+    (* start monitoring the system time *)
+    print_info (kWHT) "Client sends" (String.of_char_list (directedMsgs2string inflight));
+    let t = Prelude.Time.get_time () in
+    (* deliver the messages *)
+    let failed_to_deliver = run_replicas_on_inputs inflight in
+    (* stop monitoring the system *)
+    let d = Prelude.Time.sub_time (Prelude.Time.get_time ()) t in
+    (* calculate the average *)
+    let new_avg = Prelude.Time.div_time (Prelude.Time.add_time (Prelude.Time.mul_time avg  (timestamp - 1)) d) timestamp in
+    (* print the messages which failed to deliver as string *)
+    let s = Batteries.String.of_list (directedMsgs2string failed_to_deliver) in
+    (match s with
+     | "" -> ()
+     | s' -> print_err s');
+    (* print some results of the time is right *)
+    (if timestamp mod printing_period = 0 then
+       print_res timestamp d new_avg
+     else ());
+    (* restart the client if there are more rounds to go *)
+    if timestamp < max then
+      self#run_client (timestamp + 1) max new_avg printing_period
+    else () 
+end
+
+let _ =
+  (* create a new primary backup simulation *)
+  let c = new pb {
+    version = "1.0";
+    protocol = "PB";
+    client_id = 0;
+    private_key = lookup_client_sending_key (Obj.magic 0);
+    primary = Obj.magic PBprimary (* type: name *)
+  } in
+  c#run
+
+(* let _ = Command.run ~version:"1.0" ~build_info:"PBFT" command *)
