raft/simulator/raft/RaftReplicaEx.ml
@@ -1,0 +1,150 @@
+
+type __ = Obj.t
+
+type 'a sig0 = 'a
+  (* singleton inductive, whose constructor was exist *)
+
+
+
+(** val append : char list -> char list -> char list **)
+
+let rec append s1 s2 =
+  match s1 with
+  | [] -> s2
+  | c0::s1' -> c0::(append s1' s2)
+
+type 't deceq = bool
+
+type 't deq = 't -> 't -> 't deceq
+
+type name = __
+
+type msg = __
+
+type directedMsg = { dmMsg : msg; dmDst : name list; dmDelay : int }
+
+type directedMsgs = directedMsg list
+
+type nat_n = int
+
+type ('a, 'b) bijective =
+  'b -> 'a
+  (* singleton inductive, whose constructor was Build_bijective *)
+
+type ('s, 'i, 'o) update = 's -> 'i -> 's option * 'o
+
+type ('s, 'i, 'o) stateMachine = { sm_halted : bool;
+                                   sm_update : ('s, 'i, 'o) update;
+                                   sm_state : 's }
+
+(** val sm_halted : ('a1, 'a2, 'a3) stateMachine -> bool **)
+
+let sm_halted x = x.sm_halted
+
+(** val sm_update : ('a1, 'a2, 'a3) stateMachine -> ('a1, 'a2, 'a3) update **)
+
+let sm_update x = x.sm_update
+
+(** val sm_state : ('a1, 'a2, 'a3) stateMachine -> 'a1 **)
+
+let sm_state x = x.sm_state
+
+(** val mkSM :
+    ('a3, 'a1, 'a2) update -> 'a3 -> ('a3, 'a1, 'a2) stateMachine **)
+
+let mkSM upd s =
+  { sm_halted = false; sm_update = upd; sm_state = s }
+
+type ('s, 'i, 'o) sUpdate = 's -> 'i -> 's * 'o
+
+type 's mSUpdate = ('s, msg, directedMsgs) sUpdate
+
+(** val s2Update : ('a1, 'a2, 'a3) sUpdate -> ('a1, 'a2, 'a3) update **)
+
+let s2Update upd s i =
+  let (s', o) = upd s i in ((Some s'), o)
+
+(** val mkSSM :
+    ('a3, 'a1, 'a2) sUpdate -> 'a3 -> ('a3, 'a1, 'a2) stateMachine **)
+
+let mkSSM upd s =
+  mkSM (s2Update upd) s
+
+type 's mStateMachine = ('s, msg, directedMsgs) stateMachine
+
+(** val updState :
+    ('a1, 'a2, 'a3) stateMachine -> 'a1 -> ('a1, 'a2, 'a3) stateMachine **)
+
+let updState c0 s =
+  { sm_halted = c0.sm_halted; sm_update = c0.sm_update; sm_state = s }
+
+(** val halts :
+    ('a1, 'a2, 'a3) stateMachine -> ('a1, 'a2, 'a3) stateMachine **)
+
+let halts c0 =
+  { sm_halted = true; sm_update = c0.sm_update; sm_state = c0.sm_state }
+
+(** val force_sm :
+    ('a1, 'a2, 'a3) stateMachine -> (('a1, 'a2, 'a3) stateMachine -> 'a4) ->
+    'a4 **)
+
+let force_sm sm f0 =
+  f0 sm
+
+(** val lrun_sm :
+    ('a1, 'a2, 'a3 list) stateMachine -> 'a2 -> ('a1, 'a2, 'a3 list)
+    stateMachine * 'a3 list **)
+
+let lrun_sm c0 i =
+  if c0.sm_halted
+  then (c0, [])
+  else let (o0, o) = c0.sm_update c0.sm_state i in
+       (match o0 with
+        | Some s -> force_sm (updState c0 s) (fun sm -> (sm, o))
+        | None -> force_sm (halts c0) (fun sm -> (sm, o)))
+
+type raftcontext = { clients : int; client_deq : __ deq;
+                     clients2nat : (__ -> nat_n);
+                     clients_bji : (__, nat_n) bijective; f : int;
+                     rep_deq : __ deq; reps2nat : (__ -> nat_n);
+                     reps_bij : (__, nat_n) bijective }
+
+type c = __
+
+type raftmsg =
+| Heartbeat
+| Reply of int * c
+| Command of int
+
+type raftleader_state =
+  int
+  (* singleton inductive, whose constructor was Term *)
+
+(** val leader_update : raftcontext -> raftleader_state mSUpdate **)
+
+let leader_update _ state input =
+  match Obj.magic input with
+  | Command m -> (m, [])
+  | _ -> (state, [])
+
+(** val raftleaderSM : raftcontext -> raftleader_state mStateMachine **)
+
+let raftleaderSM raft_context =
+  mkSSM (leader_update raft_context) 0
+
+(** val str_concat : char list list -> char list **)
+
+let rec str_concat = function
+| [] -> []
+| s :: ss -> append s (str_concat ss)
+
+(** val raft_state2string : raftleader_state -> char list **)
+
+let raft_state2string _ =
+  str_concat
+    (('('::('L'::('e'::('a'::('d'::('e'::('r'::(' '::('s'::('t'::('a'::('t'::('e'::(':'::[])))))))))))))) :: ((')'::[]) :: []))
+
+(** val local_replica : raftcontext -> raftleader_state mStateMachine **)
+
+let local_replica =
+  raftleaderSM
