raft/simulator/raft/RaftReplicaEx.mli
@@ -1,0 +1,90 @@
+
+type __ = Obj.t
+
+type 'a sig0 = 'a
+  (* singleton inductive, whose constructor was exist *)
+
+
+
+val append : char list -> char list -> char list
+
+type 't deceq = bool
+
+type 't deq = 't -> 't -> 't deceq
+
+type name = __
+
+type msg = __
+
+type directedMsg = { dmMsg : msg; dmDst : name list; dmDelay : int }
+
+type directedMsgs = directedMsg list
+
+type nat_n = int
+
+type ('a, 'b) bijective =
+  'b -> 'a
+  (* singleton inductive, whose constructor was Build_bijective *)
+
+type ('s, 'i, 'o) update = 's -> 'i -> 's option * 'o
+
+type ('s, 'i, 'o) stateMachine = { sm_halted : bool;
+                                   sm_update : ('s, 'i, 'o) update;
+                                   sm_state : 's }
+
+val sm_halted : ('a1, 'a2, 'a3) stateMachine -> bool
+
+val sm_update : ('a1, 'a2, 'a3) stateMachine -> ('a1, 'a2, 'a3) update
+
+val sm_state : ('a1, 'a2, 'a3) stateMachine -> 'a1
+
+val mkSM : ('a3, 'a1, 'a2) update -> 'a3 -> ('a3, 'a1, 'a2) stateMachine
+
+type ('s, 'i, 'o) sUpdate = 's -> 'i -> 's * 'o
+
+type 's mSUpdate = ('s, msg, directedMsgs) sUpdate
+
+val s2Update : ('a1, 'a2, 'a3) sUpdate -> ('a1, 'a2, 'a3) update
+
+val mkSSM : ('a3, 'a1, 'a2) sUpdate -> 'a3 -> ('a3, 'a1, 'a2) stateMachine
+
+type 's mStateMachine = ('s, msg, directedMsgs) stateMachine
+
+val updState :
+  ('a1, 'a2, 'a3) stateMachine -> 'a1 -> ('a1, 'a2, 'a3) stateMachine
+
+val halts : ('a1, 'a2, 'a3) stateMachine -> ('a1, 'a2, 'a3) stateMachine
+
+val force_sm :
+  ('a1, 'a2, 'a3) stateMachine -> (('a1, 'a2, 'a3) stateMachine -> 'a4) -> 'a4
+
+val lrun_sm :
+  ('a1, 'a2, 'a3 list) stateMachine -> 'a2 -> ('a1, 'a2, 'a3 list)
+  stateMachine * 'a3 list
+
+type raftcontext = { clients : int; client_deq : __ deq;
+                     clients2nat : (__ -> nat_n);
+                     clients_bji : (__, nat_n) bijective; f : int;
+                     rep_deq : __ deq; reps2nat : (__ -> nat_n);
+                     reps_bij : (__, nat_n) bijective }
+
+type c = __
+
+type raftmsg =
+| Heartbeat
+| Reply of int * c
+| Command of int
+
+type raftleader_state =
+  int
+  (* singleton inductive, whose constructor was Term *)
+
+val leader_update : raftcontext -> raftleader_state mSUpdate
+
+val raftleaderSM : raftcontext -> raftleader_state mStateMachine
+
+val str_concat : char list list -> char list
+
+val raft_state2string : raftleader_state -> char list
+
+val local_replica : raftcontext -> raftleader_state mStateMachine
