raft/simulator/raft/RaftSimul.ml
@@ -1,0 +1,85 @@
+open Colors
+open Prelude
+open RsaKeyFun
+open Core
+open Simulator
+open RaftReplicaEx
+
+(* turn this to false if you don't want to sign messages *)
+let signing : bool ref = ref true
+
+let to_replica n = { id = Obj.magic (Replica (Obj.magic n));
+                     replica = local_replica (Obj.magic n) }
+let r = new replicas
+
+
+(* let sign_request breq priv =
+ *   let o  = Obj.magic (PBFTmsg_bare_request breq) in
+ *   sign_one o priv *)
+
+let destination2string (n : name) : string =
+  match Obj.magic n with
+  | Replica r -> "R(" ^ string_of_int (Obj,magic r) ^ ")"
+  | Client c -> "C(" ^ string_of_int (Obj.magic c) ^ ")";;
+
+let rec run_replicas_on_inputs (inflight : directedMsgs) : directedMsgs =
+  match inflight with
+  | [] -> []
+  | dm :: dms ->
+    (* print_info (kCYN) "Procesing" (directedMsg2string dm); *)
+    match dm.dmDst with
+    | [] -> run_replicas_on_inputs dms
+    | id :: ids ->
+      let dm' = { dmMsg = dm.dmMsg; dmDst = ids; dmDelay = dm.dmDelay } in
+      match r#find_replica id with
+      | None ->
+        print_err ("Couldn't find id " ^ destination2string id);
+        let failed_to_deliver = { dmMsg = dm.dmMsg; dmDst = [id]; dmDelay = dm.dmDelay } in
+        failed_to_deliver :: run_replicas_on_inputs (dm' :: dms)
+      | Some rep ->
+        (* print_info (kGRN) "Input message" (msg2string (Obj.magic dm.dmMsg)); *)
+        let (rep',dmsgs) = lrun_sm rep.replica (Obj.magic dm.dmMsg) in
+        print_info (kCYN) "Done" [];
+        r#replace_replica id rep';
+        run_replicas_on_inputs (dm' :: dms @ dmsgs)
+
+class ['a, 'b] pbft c = object(self)
+  inherit ['a, 'b] runner c
+
+  method create_replicas =
+    r#set_replicas [to_replica 0; to_replica 1; to_replica 2; to_replica 3];
+
+  method mk_request (timestamp : int) (request : int) =
+    let opr       = Obj.magic request in
+    (* let breq      = Bare_req (opr,timestamp,(Obj.magic c.client_id)) in *)
+    let tokens    = Obj.magic() (* [ (if !signing then Obj.magic (sign_request breq c.private_key) else Obj.magic()) ] *) in
+    Command (request)
+
+
+  method run_client timestamp max avg printing_period =
+    let req = self#mk_request (Obj.magic timestamp) 17 in
+    let inflight = [{ dmMsg = Obj.magic req; dmDst = [c.primary]; dmDelay = 0 }] in
+    let t = Prelude.Time.get_time () in
+    let failed_to_deliver = run_replicas_on_inputs inflight in
+    let d = Prelude.Time.sub_time (Prelude.Time.get_time ()) t in
+    let new_avg = Prelude.Time.div_time (Prelude.Time.add_time (Prelude.Time.mul_time avg  (timestamp - 1)) d) timestamp in
+    (*let s = Batteries.String.of_list (directedMsgs2string failed_to_deliver) in*)
+    (if timestamp mod printing_period = 0 then
+       print_res timestamp d new_avg
+     else ());
+    if timestamp < max then
+      self#run_client (timestamp + 1) max new_avg printing_period
+    else ()
+end
+
+let _ =
+  let c = new pbft {
+    version = "1.0";
+    protocol = "PBFT";
+    client_id = 0;
+    private_key = lookup_client_sending_key (Obj.magic 0);
+    primary = Obj.magic (Replica (Obj.magic 0)) (* type: name *)
+  } in
+  c#run
+
+(* let _ = Command.run ~version:"1.0" ~build_info:"PBFT" command *)
