raft/all.v
@@ -8,10 +8,7 @@
 (* Primary backup is the example implementation taken from velisarios. *)
 Require Export PrimaryBackup.
 (* the main pbft specification *)
-Require Export PBFTall.
-(* PingPong is my own dummy implementation to get a grasp on velisarios. *)
-Require Export PingPong.
+(* Require Export PBFTall. *)
 (* Raft imports the designated implementation. *)
 Require Export Raft.
 Require Export Simulator.
-
