raft/simulator/pb/PbSim.v
@@ -1,0 +1,246 @@
+(*
+ * This file defines an instance of the simple PrimaryBackup
+ * example to show the simulation of a defined protocol.
+ *)
+
+Require Export Simulator.
+Require Export Protocols.PrimaryBackup.PrimaryBackup.
+Require Export Ascii String.
+
+(* define the instance *)
+Section PrimaryBackupInstance.
+  (* simply concatenate multiple strings *)
+  Fixpoint str_concat (l : list String.string) : String.string :=
+    match l with
+    | [] => ""
+    | s :: ss => String.append s (str_concat ss)
+    end.
+
+  (* ================== TIME ================== *)
+
+  Definition time_I_type : Set := unit.
+
+  Definition time_I_get_time : unit -> time_I_type := fun _ => tt.
+
+  Definition time_I_sub : time_I_type -> time_I_type -> time_I_type := fun _ _ => tt.
+
+  Definition time_I_2string : time_I_type -> string := fun _ => "".
+
+  Global Instance TIME_I : Time.
+  Proof.
+    exists time_I_type.
+    { exact time_I_get_time. }
+    { exact time_I_sub. }
+    { exact time_I_2string. }
+  Defined.
+
+  (* ================== PRETTY PRINTING ================== *)
+
+  (* FIX: to replace when extracting *)
+  Definition print_endline : string -> unit := fun _ => tt.
+  Definition nat2string (n : nat) : string := "-".
+
+  Definition CR : string := String (ascii_of_nat 13) "".
+
+  Definition nat_n2string {m} (n : nat_n m) : string := nat2string (proj1_sig n).
+
+  Definition msg2string (m : PBmsg) : string :=
+    match m with
+    |PBinput n => str_concat ["Input ", nat2string n]
+    | PBforward n => str_concat ["Forward ", nat2string n]
+    | PBackn n => str_concat ["Ackn ", nat2string n]
+    | PBreply n => str_concat ["Reply", nat2string n]
+    end.
+
+  Definition name2string (n : PBnode) : string :=
+    match n with
+    | PBprimary => "Primary"
+    | PBbackup => "Backup"
+    | PBc => "Client"
+    end.
+
+  Fixpoint names2string (l : list PBnode) : string :=
+    match l with
+    | [] => ""
+    | [n] => name2string n
+    | n :: ns => str_concat [name2string n, ",", names2string ns]
+    end.
+
+  Definition delay2string (delay : nat) : string := nat2string delay.
+
+  Definition DirectedMsg2string (dm : DirectedMsg) : string :=
+    match dm with
+    | MkDMsg msg dst delay =>
+       str_concat ["Msg [", msg2string msg, "; Dest ", "[", names2string dst, "];", " Delay ", delay2string delay, "]"]
+    end.
+
+  Fixpoint DirectedMsgs2string (l : DirectedMsgs) : string :=
+    match l with
+    | [] => ""
+    | [dm] => DirectedMsg2string dm
+    | dm :: dmsgs => str_concat [DirectedMsg2string dm, CR, DirectedMsgs2string dmsgs]
+    end.
+
+  Definition TimedDirectedMsg2string (m : TimedDirectedMsg) : string :=
+    match m with
+    | MkTimedDMsg dm time => str_concat [DirectedMsg2string dm, ":", time_I_2string time]
+    end.
+
+  Fixpoint TimedDirectedMsgs2string (l : TimedDirectedMsgs) : string :=
+    match l with
+    | [] => ""
+    | [dm] => TimedDirectedMsg2string dm
+    | dm :: dmsgs => str_concat [TimedDirectedMsg2string dm, CR, TimedDirectedMsgs2string dmsgs]
+    end.
+
+  Definition MonoSimulationState2string (s : MonoSimulationState) : string :=
+    match s with
+    | MkMonoSimState ty sys step out_inflight in_inflight delivered =>
+      str_concat
+        [CR,
+         "====== STEP ======",
+         CR,
+         nat2string step,
+         CR,
+         "====== IN FLIGHT (from outside the system) ======",
+         CR,
+         DirectedMsgs2string out_inflight,
+         CR,
+         "====== IN FLIGHT (from inside the system) ======",
+         CR,
+         DirectedMsgs2string in_inflight,
+         CR,
+         "====== DELIVERED ======",
+         (* CR, *)
+         (* TimedDirectedMsgs2string delivered, *)
+         CR
+        ]
+    end.
+
+
+  Definition pb_state2string n :=
+    match n with
+    | PBprimary => "Primary"
+    | PBbackup => "Backup"
+    | _ => "-"
+    end.
+
+  (* ================== SYSTEM ================== *)
+
+
+  Definition dummy_initial_state : PB_state :=
+    PBbst 0.
+
+  Definition PBdummySM : MStateMachine PB_state :=
+    MhaltedSM dummy_initial_state.
+
+  Definition PBmono_sys : NMStateMachine PB_state :=
+    fun name =>
+      match name with
+      | PBprimary => PBprimarySM
+      | PBbackup => PBbackupSM
+      | _ => MhaltedSM dummy_initial_state
+      end.
+
+  Definition mk_request_to (rep : PBnode) (ts : nat) (opr : nat) : DirectedMsg :=
+    (* let ts   := time_stamp ts in *)
+    (* let breq := bare_req (opr_add opr) ts (client0 C) in *)
+    let dst  := PBprimary in (* the leader *)
+    (* let toks := [ pbft_token_stub ] : Tokens in (* we just send empty lists here to authenticate messages *) *)
+    (* let req  := req breq toks in *)
+    let msg  := PBinput opr in
+    MkDMsg msg [dst] 0.
+
+  Definition mk_request (ts : nat) (opr : nat) : DirectedMsg :=
+    mk_request_to PBprimary ts opr.
+
+  (* n request starting with number start *)
+  Fixpoint mk_requests_start (n start opr : nat) : DirectedMsgs :=
+    match n with
+    | 0 => []
+    | S m => List.app (mk_requests_start m start opr) [mk_request (n + start) opr]
+    end.
+
+  Definition mk_requests (n opr : nat) : DirectedMsgs :=
+    mk_requests_start n 0 opr.
+
+  Record InitRequests :=
+    MkInitRequests
+      {
+        num_requests     : nat;
+        starting_seq_num : nat;
+        req_operation    : nat;
+      }.
+
+  Definition PBinit_msgs (msgs : DirectedMsgs) : MonoSimulationState :=
+    MkInitMonoSimState PBmono_sys msgs.
+
+  Definition PBinit (init : InitRequests) : MonoSimulationState :=
+    PBinit_msgs
+      (mk_requests_start
+         (num_requests init)
+         (starting_seq_num init)
+         (req_operation init)).
+
+  Definition PBsimul_list (init : InitRequests) (L : list nat) : MonoSimulationState :=
+    mono_run_n_steps L (PBinit init).
+
+  Definition PBsimul_list_msgs (msgs : DirectedMsgs) (L : list nat) : MonoSimulationState :=
+    mono_run_n_steps L (PBinit_msgs msgs).
+
+  (* [switch] is the list of steps at which we want to switch to sending messages *)
+  (*  coming from the outside (from clients) instead of keeping on sending messages *)
+  (*  coming from the inside (from replicas). *)
+  Definition PBsimul_n
+             (init     : InitRequests) (* This is to generate an initial list of requests *)
+             (rounds   : Rounds)
+             (switches : Switches) : MonoSimulationState :=
+    mono_iterate_n_steps rounds switches (PBinit init).
+
+  Definition PBsimul_n_msgs
+             (msgs     : DirectedMsgs)
+             (rounds   : Rounds)
+             (switches : Switches) : MonoSimulationState :=
+    mono_iterate_n_steps rounds switches (PBinit_msgs msgs).
+
+End PrimaryBackupInstance.
+
+(* ================== EXTRACTION ================== *)
+
+
+Extraction Language Ocaml.
+
+(* printing stuff *)
+Extract Inlined Constant print_endline => "Prelude.print_coq_endline".
+Extract Inlined Constant nat2string    => "Prelude.char_list_of_int".
+Extract Inlined Constant CR            => "['\n']".
+
+(* numbers *)
+Extract Inlined Constant Nat.modulo    => "(mod)".
+
+(* lists *)
+Extract Inlined Constant forallb => "List.for_all".
+Extract Inlined Constant existsb => "List.exists".
+Extract Inlined Constant length  => "List.length".
+Extract Inlined Constant app     => "List.append".
+Extract Inlined Constant map     => "List.map".
+Extract Inlined Constant filter  => "List.filter".
+
+(* timing stuff *)
+Extract Inlined Constant time_I_type     => "float".
+Extract Inlined Constant time_I_get_time => "Prelude.Time.get_time".
+Extract Inlined Constant time_I_sub      => "Prelude.Time.sub_time".
+Extract Inlined Constant time_I_2string  => "Prelude.Time.time2string".
+
+Require Export ExtrOcamlBasic.
+Require Export ExtrOcamlNatInt.
+Require Export ExtrOcamlString.
+
+Definition local_replica (n : name) :=
+  match n with
+  | PBprimary => @PBprimarySM
+  | PBbackup => @PBbackupSM
+  | _ => @PBbackupSM
+  end.
+
+Extraction "PbReplicaEx.ml" pb_state2string lrun_sm MonoSimulationState2string PBdummySM local_replica.
