raft/simulator/raft/RaftSim.v
@@ -1,0 +1,723 @@
+(*
+ * This file defines an instance of the simple PrimaryBackup
+ * example to show the simulation of a defined protocol.
+ *)
+
+Require Export Simulator.
+Require Export Protocols.Raft.Raft.
+Require Export Ascii String.
+
+(* define some instance of raft *)
+Section RaftInstance.
+
+  (* ================== TIME ================== *)
+
+
+  Definition time_I_type : Set := unit.
+
+  Definition time_I_get_time : unit -> time_I_type := fun _ => tt.
+
+  Definition time_I_sub : time_I_type -> time_I_type -> time_I_type := fun _ _ => tt.
+
+  Definition time_I_2string : time_I_type -> string := fun _ => "".
+
+  Global Instance TIME_I : Time.
+  Proof.
+    exists time_I_type.
+    { exact time_I_get_time. }
+    { exact time_I_sub. }
+    { exact time_I_2string. }
+  Defined.
+
+
+  (* total number of faults *)
+  Definition F := 1.
+
+  (* total number of clients which is c + 1 *)
+  Definition C := 0.
+
+  (* maximum requests in progress *)
+  Definition MIP := 2.
+
+   (* define the key exchange and authentication *)
+  Definition raft_digest : Set := list nat.
+
+  Lemma raft_digest_deq : Deq raft_digest.
+  Proof.
+    introv; apply list_eq_dec.
+    apply deq_nat.
+  Defined.
+
+  Inductive sending_key_stub : Set :=
+  | raft_sending_key_stub.
+
+  Inductive receiving_key_stub : Set :=
+  | raft_receiving_key_stub.
+
+  Definition raft_sending_key   : Set := sending_key_stub.
+  Definition raft_receiving_key : Set := receiving_key_stub.
+
+  (* define the number of replicas as 3 time the number of faults happening plus one *)
+  Definition nreps (F : nat) : nat := 3 * F + 1.
+
+  (* declare the set of replicas *)
+  Definition replica (F : nat) : Set := nat_n (nreps F).
+
+  Lemma replica_deq (F : nat) : Deq (replica F).
+  Proof.
+    apply nat_n_deq.
+  Defined.
+
+  (* convert between the replica and the number indicating the replica *)
+  Definition reps2nat (F : nat) : replica F -> nat_n (nreps F) := fun n => n.
+
+  
+  Lemma bijective_reps2nat (F : nat) : bijective (reps2nat F).
+  Proof.
+    exists (fun n : nat_n (nreps F) => n); introv; unfold reps2nat; auto.
+  Defined.
+
+  (* define the number of clients *)
+  Definition nclients (C : nat) : nat := S C.
+
+  (* create the set of clients *)
+  Definition client (C : nat) : Set := nat_n (nclients C).
+
+  Definition client0 (C : nat) : client C.
+  Proof.
+    exists 0.
+    apply leb_correct.
+    unfold nclients.
+    omega.
+  Defined.
+
+  Lemma client_deq (C : nat) : Deq (client C).
+  Proof.
+    apply nat_n_deq.
+  Defined.
+
+  (* convert between a client and the numeral representation *)
+  Definition clients2nat (C : nat) : client C -> nat_n (nclients C) := fun n => n.
+
+  Lemma bijective_clients2nat (C : nat) : bijective (clients2nat C).
+  Proof.
+    exists (fun n : nat_n (nclients C) => n); introv; unfold clients2nat; auto.
+  Defined.
+
+  Global Instance Ract_I_context : Raftcontext :=
+    MkRaftContext
+      (nclients C)
+      (client C)
+      (client_deq C)
+      (clients2nat C)
+      (bijective_clients2nat C)
+
+      F
+      (replica F)
+      (replica_deq F)
+      (reps2nat F)
+      (bijective_reps2nat F).
+
+
+ 
+  (* define some client operations *)
+  Inductive operation :=
+  | opr_add (n : nat)
+  | opr_sub (n : nat).
+
+  Lemma operation_deq : Deq operation.
+  Proof.
+    introv; destruct x as [n|n], y as [m|m]; prove_dec;
+      destruct (deq_nat n m); subst; prove_dec.
+  Defined.
+
+  Definition smState : Set := nat.
+  Definition result : Set := nat.
+
+  Definition operation_upd (C : nat) (c : client C) (state : smState) (opr : operation) : result * smState :=
+    match opr with
+    | opr_add m => let k := state + m in (k,k)
+    | opr_sub m => let k := state - m in (k,k)
+    end.
+
+  Inductive Rafttoken_stub : Set :=
+  | raft_token_stub.
+
+  Definition raft_token : Set := Rafttoken_stub.
+
+  Lemma raft_token_deq : Deq raft_token.
+  Proof.
+    introv; destruct x, y; simpl; prove_dec.
+  Defined.
+
+
+  (* authentication stuff *)
+  (* Definition raft_create_signature *)
+  (*            (m  : Raftmsg) *)
+  (*            (ks : sending_keys) : Rafttokens := [raft_token_stub]. *)
+
+  (* Definition raft_verify_signature *)
+  (*            (m : PBFTBare_Msg) *)
+  (*            (n : name) *)
+  (*            (k : receiving_key) *)
+  (*            (a : raft_token) : bool := true. *)
+
+  (* Global Instance PB_I_auth : PBauth := *)
+  (*   MkPBauth pb_create_signature pb_verify_signature. *)
+
+
+  (* Definition pb_lookup_replica_sending_key   (src : Rep)    : pb_sending_key   := pb_sending_key_stub. *)
+  (* Definition pb_lookup_replica_receiving_key (dst : Rep)    : pb_receiving_key := pb_receiving_key_stub. *)
+  (* Definition pb_lookup_client_receiving_key  (c   : Client) : pb_receiving_key := pb_receiving_key_stub. *)
+
+  (* Definition initial_pb_local_key_map_replicas (src : name) : local_key_map := *)
+  (*   match src with *)
+  (*   | PBbackup => *)
+  (*     MkLocalKeyMap *)
+  (*       [MkDSKey (map PBprimary reps) (pb_lookup_replica_sending_key i)] *)
+  (*       (List.app *)
+  (*          (map (fun c => MkDRKey [PBc] (pb_lookup_client_receiving_key  c)) clients) *)
+  (*          (map (fun m => MkDRKey [PBbackup] (pb_lookup_replica_receiving_key m) nreps))) *)
+  (*   | PBc => MkLocalKeyMap [] [] *)
+  (*   end. *)
+
+  (* Global Instance PB_I_keys : PBinitial_keys := *)
+  (*   MkPBinitial_keys initial_pb_local_key_map_replicas. *)
+  
+  (* Definition pb_simple_create_hash_messages (msgs : list PBmsg) : PBdigest := []. *)
+  (* Definition pb_simple_verify_hash_messages (msgs : list PBmsg) (d : PBdigest) := true. *)
+  (* Definition pb_simple_create_hash_state_last_reply (smst : PBsm_state) (lastr : LastReplyState) : PBdigest := []. *)
+  (* Definition pb_simple_verify_hash_state_last_reply (smst : PBsm_state) (lastr : LastReplyState) (d : PBdigest) := true. *)
+
+  (* Global Instance PB_I_hash : PBhash := *)
+  (*   MkPBhash *)
+  (*     pb_simple_create_hash_messages *)
+  (*     pb_simple_verify_hash_messages *)
+  (*     pb_simple_create_hash_state_last_reply *)
+  (*     pb_simple_verify_hash_state_last_reply. *)
+
+
+  (* Global Instance PB_I_context : PBcontext := *)
+  (*   MkPBcontext *)
+  (*     (* max in progress *) *)
+  (*     MIP *)
+
+  (*     (* water mark range *) *)
+  (*     WMR *)
+
+  (*     (* checkpoint period *) *)
+  (*     CP *)
+
+  (*     (* digest type *) *)
+  (*     pb_digest *)
+
+  (*     (* digest decider *) *)
+  (*     pb_digest_deq *)
+
+  (*     (* token type *) *)
+  (*     pb_token *)
+
+  (*     (* token decider *) *)
+  (*     pb_token_deq *)
+
+  (*     (* sending key type *) *)
+  (*     pb_sending_key *)
+
+  (*     (* receiving key type *) *)
+  (*     pb_receiving_key *)
+
+  (*     (* number of faults *) *)
+  (*     F *)
+
+  (*     (* replica type *) *)
+  (*     (replica F) *)
+
+  (*     (* Replica decider *) *)
+  (*     (replica_deq F) *)
+
+  (*     (* replica 2 nat *) *)
+  (*     (reps2nat F) *)
+
+  (*     (* proof that reps2nat is bijective *) *)
+  (*     (bijective_reps2nat F) *)
+
+  (*     (* number of clients *) *)
+  (*     (nclients C) *)
+
+  (*     (* client type *) *)
+  (*     (client C) *)
+
+  (*     (* client decider *) *)
+  (*     (client_deq C) *)
+
+  (*     (* client 2 nat *) *)
+  (*     (clients2nat C) *)
+
+  (*     (* proof that clients2nat is bijective *) *)
+  (*     (bijective_clients2nat C) *)
+
+  (*     (* operation type *) *)
+  (*     operation *)
+
+  (*     (* operation decider *) *)
+  (*     operation_deq *)
+
+  (*     (* result type *) *)
+  (*     result *)
+
+  (*     (* result decider *) *)
+  (*     deq_nat *)
+
+  (*     (* state type *) *)
+  (*     smState *)
+
+  (*     (* initial state *) *)
+  (*     0 *)
+
+  (*     (* update function *) *)
+  (*     (operation_upd C) *)
+
+  (*     (* delay in ms *) *)
+  (*     1000. *)
+
+  (* ================== PRETTY PRINTING ================== *)
+
+    Fixpoint str_concat (l : list String.string) : String.string :=
+    match l with
+    | [] => ""
+    | s :: ss => String.append s (str_concat ss)
+    end.
+
+  (* FIX: to replace when extracting *)
+  Definition print_endline : string -> unit := fun _ => tt.
+  Definition nat2string (n : nat) : string := "-".
+
+  Definition CR : string := String (ascii_of_nat 13) "".
+
+  (* Fix: to finish *)
+  (*Definition tokens2string (toks : Tokens) : string := "-".
+*)
+  (* Fix: to finish *)
+  Definition digest2string (d : raft_digest) : string := "-".
+
+  (* Fix: to finish *)
+  Definition result2string (r : result) : string := "-".
+
+  (* Fix: there's only one client anyway *)
+  Definition client2string (c : client C) : string := "-".
+
+  (* Definition timestamp2string (ts : Timestamp) : string := *)
+  (*   match ts with *)
+  (*   | time_stamp n => nat2string n *)
+  (*   end. *)
+
+  (*Definition view2string (v : View) : string :=
+    match v with
+    | view n => nat2string n
+    end.
+*)
+  (*Definition seq2string (s : SeqNum) : string :=
+    match s with
+    | seq_num n => nat2string n
+    end.
+*)
+  (* Definition operation2string (opr : operation) : string := *)
+  (*   match opr with *)
+  (*   | opr_add n => str_concat ["+", nat2string n] *)
+  (*   | opr_sub n => str_concat ["-", nat2string n] *)
+  (*   end. *)
+
+  Definition nat_n2string {m} (n : nat_n m) : string := nat2string (proj1_sig n).
+
+  Definition replica2string (r : replica F) : string := nat_n2string r.
+
+(*  Definition bare_request2string (br : Bare_Request) : string :=
+    match br with
+    | null_req => str_concat [ "null_req"]
+    | bare_req opr ts c => str_concat [operation2string opr, ",", timestamp2string ts, ",", client2string c]
+    end.
+
+  Definition request2string (r : Request) : string :=
+    match r with
+    | req br a => str_concat ["REQUEST(", bare_request2string br, ",", tokens2string a, ")"]
+    end.
+
+  Fixpoint requests2string (rs : list Request) : string :=
+    match rs with
+    | [] => ""
+    | [r] => request2string r
+    | r :: rs => str_concat [request2string r, ",", requests2string rs]
+    end.
+
+  Definition bare_pre_prepare2string (bpp : Bare_Pre_prepare) : string :=
+    match bpp with
+    | bare_pre_prepare v s reqs => str_concat [view2string v, ",", seq2string s, ",", requests2string reqs]
+    end.
+
+  Definition bare_prepare2string (bp : Bare_Prepare) : string :=
+    match bp with
+    | bare_prepare v s d i => str_concat [view2string v, ",", seq2string s, ",", digest2string d, ",", replica2string i]
+    end.
+
+  Definition bare_commit2string (bc : Bare_Commit) : string :=
+    match bc with
+    | bare_commit v s d i => str_concat [view2string v, ",", seq2string s, ",", digest2string d, ",", replica2string i]
+    end.
+
+  Definition bare_reply2string (br : Bare_Reply) : string :=
+    match br with
+    | bare_reply v ts c i res => str_concat [view2string v, ",", timestamp2string ts, ",", client2string c, ",", replica2string i, ",", result2string res]
+    end.
+
+  Definition pre_prepare2string (pp : Pre_prepare) : string :=
+    match pp with
+    | pre_prepare b a => str_concat ["PRE_PREPARE(",bare_pre_prepare2string b, ",", tokens2string a, ")"]
+    end.
+
+  Definition prepare2string (p : Prepare) : string :=
+    match p with
+    | prepare bp a => str_concat ["PREPARE(", bare_prepare2string bp, ",", tokens2string a, ")"]
+    end.
+
+  Definition commit2string (c : Commit) : string :=
+    match c with
+    | commit bc a => str_concat ["COMMIT(", bare_commit2string bc, ",", tokens2string a, ")"]
+    end.
+
+  Definition reply2string (r : Reply) : string :=
+    match r with
+    | reply br a => str_concat ["REPLY(", bare_reply2string br, ",", tokens2string a, ")"]
+    end.
+
+  Definition debug2string (d : Debug) : string :=
+    match d with
+    | debug r s => str_concat ["DEBUG(", replica2string r, ",", s, ")"]
+    end.
+
+  Definition bare_checkpoint2string (bc : Bare_Checkpoint) : string :=
+    match bc with
+    | bare_checkpoint v n d i => str_concat [view2string v, ",", seq2string n, ",", digest2string d, ",", replica2string i]
+    end.
+
+  Definition checkpoint2string (c : Checkpoint) : string :=
+    match c with
+    | checkpoint bc a => str_concat ["CHECKPOINT(", bare_checkpoint2string bc, ",", tokens2string a, ")"]
+    end.
+
+  Definition check_ready2string (c : CheckReady) : string := "CHECK-READY()".
+
+  Definition check_stable2string (c : CheckStableChkPt) : string := "CHECK-STABLE()".
+
+  Definition start_timer2string (t : StartTimer) : string :=
+    match t with
+    | start_timer r v => str_concat ["START-TIMER(", bare_request2string r, "," , view2string v, ")"]
+    end.
+
+  Definition expired_timer2string (t : ExpiredTimer) : string :=
+    match t with
+    | expired_timer r v => str_concat ["EXPIRED-TIMER(", bare_request2string r, "," , view2string v, ")"]
+    end.
+
+  (* FIX *)
+  Definition stable_chkpt2string (stable : StableChkPt) : string := "-".
+
+  (* FIX *)
+  Definition checkpoint_cert2string (cert : CheckpointCert) : string := "-".
+
+  (* FIX *)
+  Definition prepared_infos2string (l : list PreparedInfo) : string := "-".
+
+  Definition bare_view_change2string (bvc : Bare_ViewChange) : string :=
+    match bvc with
+    | bare_view_change v n stable cert preps i =>
+      str_concat
+        [view2string v,
+         ",",
+         seq2string n,
+         ",",
+         stable_chkpt2string stable,
+         ",",
+         checkpoint_cert2string cert,
+         ",",
+         prepared_infos2string preps,
+         ",",
+         replica2string i
+        ]
+    end.
+
+  Definition view_change2string (vc : ViewChange) : string :=
+    match vc with
+    | view_change bvc a => str_concat ["VIEW-CHANGE(", bare_view_change2string bvc, ",", tokens2string a, ")"]
+    end.
+
+  (* FIX *)
+  Definition view_change_cert2string (V : ViewChangeCert) : string := "-".
+
+  Fixpoint pre_prepares2string (l : list Pre_prepare) : string :=
+    match l with
+    | [] => ""
+    | [r] => pre_prepare2string r
+    | r :: rs => str_concat [pre_prepare2string r, ",", pre_prepares2string rs]
+    end.
+
+  Definition bare_new_view2string (bnv : Bare_NewView) : string :=
+    match bnv with
+    | bare_new_view v V OP NP =>
+      str_concat
+        [
+          view2string v,
+          ",",
+          view_change_cert2string V,
+          ",",
+          pre_prepares2string OP,
+          ",",
+          pre_prepares2string NP
+        ]
+    end.
+
+  Definition new_view2string (nv : NewView) : string :=
+    match nv with
+    | new_view bnv a => str_concat ["NEW-VIEW(", bare_new_view2string bnv, ",", tokens2string a, ")"]
+    end.
+
+  Definition check_bcast_new_view2string (c : CheckBCastNewView) : string :=
+    match c with
+    | check_bcast_new_view i => str_concat ["CHECK-BCAST-NEW-VIEW(", nat2string i, ")"]
+    end.
+
+  Definition msg2string (m : PBFTmsg) : string :=
+    match m with
+    | PBFTrequest r              => request2string r
+    | PBFTpre_prepare pp         => pre_prepare2string pp
+    | PBFTprepare p              => prepare2string p
+    | PBFTcommit c               => commit2string c
+    | PBFTcheckpoint c           => checkpoint2string c
+    | PBFTcheck_ready c          => check_ready2string c
+    | PBFTcheck_stable c         => check_stable2string c
+    | PBFTcheck_bcast_new_view c => check_bcast_new_view2string c
+    | PBFTstart_timer t          => start_timer2string t
+    | PBFTexpired_timer t        => expired_timer2string t
+    | PBFTview_change v          => view_change2string v
+    | PBFTnew_view v             => new_view2string v
+    | PBFTdebug d                => debug2string d
+    | PBFTreply r                => reply2string r
+    end.
+*)
+  (* Definition name2string (n : name) : string := *)
+  (*   match n with *)
+  (*   | Raftleader => "leader" *)
+  (*   end. *)
+
+  (* Fixpoint names2string (l : list name) : string := *)
+  (*   match l with *)
+  (*   | [] => "" *)
+  (*   | [n] => name2string n *)
+  (*   | n :: ns => str_concat [name2string n, ",", names2string ns] *)
+  (*   end. *)
+
+  (* Definition delay2string (delay : nat) : string := nat2string delay. *)
+
+  Definition msg2string (m : Raftmsg) : string :=
+    match m with
+    | Command n => "Command " ++ nat2string n
+    | _ => "Other msg"
+    end.
+
+  (* Definition DirectedMsg2strking (dm : DirectedMsg) : string := *)
+  (*   match dm with *)
+  (*   | MkDMsg msg dst delay =>  *)
+  (*     (* concat ["msg", ":", "[", " dest" , "]", ":"] *) *)
+  (*   end. *)
+
+  (* Fixpoint DirectedMsgs2string (l : DirectedMsgs) : string := *)
+  (*   match l with *)
+  (*   | [] => "" *)
+  (*   | [dm] => "msg" (* DirectedMsg2string dm *) *)
+  (*   | dm :: dmsgs => str_concat ["mutliple msgs"] (* [DirectedMsg2string dm, CR, DirectedMsgs2string dmsgs] *) *)
+  (*   end. *)
+(*
+  Definition TimedDirectedMsg2string (m : TimedDirectedMsg) : string :=
+    match m with
+    | MkTimedDMsg dm time => str_concat [DirectedMsg2string dm, ":", time_I_2string time]
+    end.
+
+  Fixpoint TimedDirectedMsgs2string (l : TimedDirectedMsgs) : string :=
+    match l with
+    | [] => ""
+    | [dm] => TimedDirectedMsg2string dm
+    | dm :: dmsgs => str_concat [TimedDirectedMsg2string dm, CR, TimedDirectedMsgs2string dmsgs]
+    end.
+*)
+(*   Definition MonoSimulationState2string (s : MonoSimulationState) : string := *)
+(*     match s with *)
+(*     | MkMonoSimState ty sys step out_inflight in_inflight delivered => *)
+(*       concat *)
+(*         [CR, *)
+(*           "====== STEP ======", *)
+(*           CR, *)
+(*           nat2string step, *)
+(*           CR, *)
+(*           "====== IN FLIGHT (from outside the system) ======", *)
+(*           CR, *)
+(*           (*DirectedMsgs2string out_inflight,*) *)
+(*           CR, *)
+(*           "====== IN FLIGHT (from inside the system) ======", *)
+(*           CR, *)
+(*           (*DirectedMsgs2string in_inflight,*) *)
+(*           CR, *)
+(*           "====== DELIVERED ======" *)
+(* (*CR, *)
+(*          TimedDirectedMsgs2string delivered, *)
+(*          CR*) *)
+(*         ] *)
+(*     end. *)
+ 
+
+
+
+  Definition raft_state2string (s : Raftleader_state) :=
+      str_concat
+        ["(Leader state:"
+         ,")"
+        ].
+
+  (* ================== SYSTEM ================== *)
+
+  
+
+  (* Definition dummy_initial_state : Raftnode := *)
+  (*    Replica . *)
+
+  (* Definition RaftdummySM : MStateMachine Raftnode := *)
+  (*   MhaltedSM dummy_initial_state. *)
+
+  (* Definition PBFTmono_sys : NMStateMachine Raftnode := *)
+  (*   fun name => *)
+  (*     match name with *)
+  (*     | Leader => RaftleaderSM *)
+  (*     (* | _ => MhaltedSM dummy_initial_state *) *)
+  (*     end. *)
+
+  (* Definition mk_request_to (rep : Rep) (ts : nat) (opr : nat) : DirectedMsg := *)
+  (*   let ts   := time_stamp ts in *)
+  (*   let breq := bare_req (opr_add opr) ts (client0 C) in *)
+  (*   let dst  := PBFTreplica rep in (* the leader *) *)
+  (*   let toks := [ pbft_token_stub ] : Tokens in (* we just send empty lists here to authenticate messages *) *)
+  (*   let req  := req breq toks in *)
+  (*   let msg  := PBFTrequest req in *)
+  (*   MkDMsg msg [dst] 0. *)
+
+  (* Definition mk_request (ts : nat) (opr : nat) : DirectedMsg := *)
+  (*   mk_request_to (PBFTprimary initial_view) ts opr. *)
+
+  (* (* n request starting with number start *) *)
+  (* Fixpoint mk_requests_start (n start opr : nat) : DirectedMsgs := *)
+  (*   match n with *)
+  (*   | 0 => [] *)
+  (*   | S m => List.app (mk_requests_start m start opr) [mk_request (n + start) opr] *)
+  (*   end. *)
+
+  (* Definition mk_requests (n opr : nat) : DirectedMsgs := *)
+  (*   mk_requests_start n 0 opr. *)
+
+  (* Record InitRequests := *)
+  (*   MkInitRequests *)
+  (*     { *)
+  (*       num_requests     : nat; *)
+  (*       starting_seq_num : nat; *)
+  (*       req_operation    : nat; *)
+  (*     }. *)
+
+  (* Definition PBFTinit_msgs (msgs : DirectedMsgs) : MonoSimulationState := *)
+  (*   MkInitMonoSimState PBFTmono_sys msgs. *)
+
+  (* Definition PBFTinit (init : InitRequests) : MonoSimulationState := *)
+  (*   PBFTinit_msgs *)
+  (*     (mk_requests_start *)
+  (*        (num_requests init) *)
+  (*        (starting_seq_num init) *)
+  (*        (req_operation init)). *)
+
+  (* Definition PBFTsimul_list (init : InitRequests) (L : list nat) : MonoSimulationState := *)
+  (*   mono_run_n_steps L (PBFTinit init). *)
+
+  (* Definition PBFTsimul_list_msgs (msgs : DirectedMsgs) (L : list nat) : MonoSimulationState := *)
+  (*   mono_run_n_steps L (PBFTinit_msgs msgs). *)
+
+  (* (* [switch] is the list of steps at which we want to switch to sending messages *)
+  (*  coming from the outside (from clients) instead of keeping on sending messages *)
+  (*  coming from the inside (from replicas). *) *)
+  (* Definition PBFTsimul_n *)
+  (*            (init     : InitRequests) (* This is to generate an initial list of requests *) *)
+  (*            (rounds   : Rounds) *)
+  (*            (switches : Switches) : MonoSimulationState := *)
+  (*   mono_iterate_n_steps rounds switches (PBFTinit init). *)
+
+  (* Definition PBFTsimul_n_msgs *)
+  (*            (msgs     : DirectedMsgs) *)
+  (*            (rounds   : Rounds) *)
+  (*            (switches : Switches) : MonoSimulationState := *)
+  (*   mono_iterate_n_steps rounds switches (PBFTinit_msgs msgs). *)
+
+End RaftInstance.
+
+
+(* ================== EXTRACTION ================== *)
+
+
+Extraction Language Ocaml.
+
+(* printing stuff *)
+Extract Inlined Constant print_endline => "Prelude.print_coq_endline".
+Extract Inlined Constant nat2string    => "Prelude.char_list_of_int".
+
+(* numbers *)
+Extract Inlined Constant Nat.modulo    => "(mod)".
+
+(* lists *)
+Extract Inlined Constant forallb => "List.for_all".
+Extract Inlined Constant existsb => "List.exists".
+Extract Inlined Constant length  => "List.length".
+Extract Inlined Constant app     => "List.append".
+Extract Inlined Constant map     => "List.map".
+Extract Inlined Constant filter  => "List.filter".
+
+(* timing stuff *)
+Extract Inlined Constant time_I_type     => "float".
+Extract Inlined Constant time_I_get_time => "Prelude.Time.get_time".
+Extract Inlined Constant time_I_sub      => "Prelude.Time.sub_time".
+Extract Inlined Constant time_I_2string  => "Prelude.Time.time2string".
+
+
+(* == crypto stuff == *)
+(* === COMMENT OUT THIS PART IF YOU DON'T WANT TO USE KEYS === *)
+(* Extract Inlined Constant raft_sending_key   => "Nocrypto.Rsa.priv". *)
+(* Extract Inlined Constant raft_receiving_key => "Nocrypto.Rsa.pub". *)
+(* Extract Inlined Constant raft_lookup_replica_sending_key   => "RsaKeyFun.lookup_replica_sending_key". *)
+(* Extract Inlined Constant raft_lookup_replica_receiving_key => "RsaKeyFun.lookup_replica_receiving_key". *)
+(* Extract Inlined Constant raft_lookup_client_receiving_key  => "RsaKeyFun.lookup_client_receiving_key". *)
+
+(* Extract Inlined Constant raft_create_signature => "RsaKeyFun.sign_list". *)
+(* Extract Inlined Constant raft_verify_signature => "RsaKeyFun.verify_one". *)
+(* Extract Inlined Constant raft_token => "Cstruct.t". *)
+(* Extract Inlined Constant raft_token_deq => "(=)". *)
+(* === --- === *)
+
+
+(* == hashing stuff == *)
+(* Extract Inlined Constant raft_digest => "Cstruct.t". *)
+(* Extract Inlined Constant raft_digest_deq => "(=)". *)
+(* Extract Inlined Constant raft_simple_create_hash_messages => "Obj.magic (Hash.create_hash_objects)". *)
+(* Extract Inlined Constant raft_simple_verify_hash_messages => "Obj.magic (Hash.verify_hash_objects)". *)
+(* Extract Inlined Constant raft_simple_create_hash_state_last_reply => "Obj.magic (Hash.create_hash_pair)". *)
+(* Extract Inlined Constant raft_simple_verify_hash_state_last_reply => "Obj.magic (Hash.verify_hash_pair)". *)
+(* === --- === *)
+
+Require Export ExtrOcamlBasic.
+Require Export ExtrOcamlNatInt.
+Require Export ExtrOcamlString.
+
+Definition local_replica (*(F C : nat)*) :=
+  @RaftleaderSM.
+   
+Extraction "raft/RaftReplicaEx.ml" raft_state2string lrun_sm  RaftleaderSM local_replica.
